added compact printing in the SquiggleEq library.
used it to define compact (not necessarily pretty) printing for L4a.
(also updated SquiggleEq to the latest version fef0f1dfacc6b636a129558ee8e9836eb77476f1)
Although it produces decent results on simple examples, it
runs into stack overflow when printing Gcd (compiled to L4a).

Also, Quoting Gcd is very slow -- takes almost a minute.
In contrast, Extraction is very fast on Gcd.

libraries/SquiggleEq/terms.v
@@ -34,6 +34,7 @@ Generalizable Variable Opid.
 
 Section terms.
 
+
 Context {NVar VarClass} `{VarType NVar VarClass} `{Deq Opid} {gts : GenericTermSig Opid}.
 
 Inductive NTerm : Type :=
@@ -96,6 +97,12 @@ Definition isvariable (t : NTerm) :=
     | vterm _ => True
     | _ => False
   end.
+
+Definition getOpid (n: NTerm) : option Opid :=
+match n with
+| vterm _ => None
+| oterm o _ => Some o
+end. 
 
 
 (*Notation "x # b" := (bterm [x] b) (at level 70, right associativity).
@@ -250,3 +257,64 @@ Definition closed (t : @NTerm NVar Opid) := free_vars t = [].
 Definition isprogram (t : @NTerm NVar Opid) := closed t # nt_wf t.
 
 End termsCont.
+
+Fixpoint tmap {V1 V2 O1 O2  :Type} (fv: V1 -> V2) (fo : O1 -> O2) (t : @NTerm V1 O1) 
+  : (@NTerm V2 O2) :=
+match t with
+| vterm v =>  vterm (fv v)
+| oterm o lbt => oterm (fo o) (map (tmap_bterm fv fo) lbt)
+end
+with 
+tmap_bterm {V1 V2 O1 O2  :Type} (fv: V1 -> V2) (fo : O1 -> O2) (t : @BTerm V1 O1) 
+  : (@BTerm V2 O2) :=
+match t with
+| bterm lv nt => bterm (map fv lv) (tmap fv fo nt)
+end.
+
+Definition tvmap {V1 V2 O  :Type} (fv: V1 -> V2) : (@NTerm V1 O) -> (@NTerm V2 O) :=
+tmap fv id.
+
+
+Require Import String.
+
+SearchAbout (list string -> string).
+
+
+Definition flatten (l:list string) : string :=
+  List.fold_left append  l EmptyString.
+
+Fixpoint flattenDelim (d:string) (l:list string) {struct l}: string :=
+match l with 
+| nil => EmptyString
+| h::tl => match tl with
+          | nil => h
+          | m::tm => flatten [h;d; flattenDelim d tl]
+          end
+end.
+(*
+Eval vm_compute in (flattenDelim "," []).
+Eval vm_compute in (flattenDelim "," ["hello"]).
+Eval vm_compute in (flattenDelim "," ["hello"; "how"]).
+Eval vm_compute in (flattenDelim "," ["hello"; "how" ; "are"]).
+*)
+
+Definition newLineChar : Ascii.ascii := Ascii.ascii_of_nat 10.
+Definition newLineString : string := String newLineChar EmptyString.
+
+Fixpoint tprint {V O  :Type} (spaces:string) (fv: V -> string) (fo : O -> string) (t : @NTerm V O) 
+  : string :=
+match t with
+| vterm v =>  flatten [fv v; newLineString]
+| oterm o lbt => 
+  flatten [(fo o); newLineString; flatten (map (bprint (append " " spaces) fv fo) lbt)]
+end
+with 
+bprint {V O  :Type} (spaces:string) (fv: V -> string) (fo : O -> string) (t : @BTerm V O) 
+  : string :=
+match t with
+| bterm lv nt =>  
+  let pv := flattenDelim " " (map fv lv) in
+  let pt := tprint spaces fv fo nt in
+    flatten [spaces; pv; "." ; pt]
+end.
+
