libraries/SquiggleEq/export.v
@@ -4,3 +4,9 @@ Require Export terms2.
 Require Export substitution.
 Require Export alphaeq.
 
+
+Require Import List.
+
+
+
+
